\subsection*{Model Parameter Definitions}
\begin{itemize}
\item Parameters of the nonlinear model (equation~\ref{eqn::full_nonlinear})
\begin{align*}
    \footnotesize
    &\mat{
    \\f_{13} &=& k_1
    \\f_{23} &=& k_{4F}
    \\f_{32} &=& k_{4F} \Theta
    \\f_{31} &=& k_1 V
    \\f_{24} &=& b_v f_v
    \\b_{11} &=& b_v f_v
    },
    \qquad \qquad \qquad
    \mat{
    \\ g_1    &=& b_v f_v
    \\ g_2    &=& b_v f_v + k_{4F} \Theta
    \\ g_{3}  &=& k_{4R}+k_3
    \\ g_{23} &=& k_{4R} V^{-1}
    \\ g_{32} &=& k_{4F} V \Theta
    \\ g_4 &=& \omega_u
    \\ b_{42} &=& \frac{\omega_u b_u}{f_v}
    }
\end{align*}
%===============================================================================
\item Parameters of the linear model (equation~\ref{eqn::lin_model})

\begin{minipage}{0.49 \textwidth}
\begin{align*}
    \footnotesize
    a_{11} &= -\lr{ \bar f_{13} \bar x_3 + \bar g_1 } \\
    a_{22} &= \lr{ -\bar g_2 + \bar f_{23} \bar x_3 } \\
    a_{23} &= \lr{\bar f_{23} \bar x_2 + \bar g_{23}} \\
    a_{32} &= \lr{-\bar f_{32} \bar x_3 + \bar g_{32} } \\
    a_{33} &= \lr{-\bar f_{32} \bar x_2 - \bar g_3 - \bar f_{31} \bar x_1}  \\
    b_{23} &= -\delta g_{2_T} \bar x_2 + \delta f_{23} \bar x_2 \bar x_3 + \delta g_{23} \bar x_3 \\
    b_{33} &= -\delta f_{32} \bar x_2 \bar x_3 - \delta g_3 \bar x_3 - \delta f_{31} \bar x_1 \bar x_3 + \delta g_{32} \bar x_2 \\
    b_{14} &= \lr{\delta b_{11} \bar u_1- \delta g_1 \bar x_1} \\
    b_{24} &= \lr{-\delta g_{2_F} \bar x_2 + \delta f_{24} \bar x_4 }\\
    %===
\end{align*}
\end{minipage}
\begin{minipage}{0.49\textwidth}
\begin{align*}
    \footnotesize
    %===
    \bar f_{13} &= \bar k_{1}, \quad
    \delta f_{13}  = \lr{ p_{1} \bar k_{1} } \\
    %===
    \bar f_{23} &= \bar k_{4F}, \quad
    \delta f_{23} = \lr{ p_{4F} \bar k_{4F} } \\
    %===
    \bar f_{32} &= \bar k_{4F} \Theta, \quad
    \delta f_{32}  = \lr{ p_{4F}  \bar k_{4F} \Theta }
    \\
    \bar f_{31} &= \bar k_1 V, \quad
    \delta f_{31}  = \lr{ p_1 \bar k_1 V }
    \\
    \bar f_{24} &= b_v \bar f_v,
    \quad
    \delta f_{24}  = b_v
    \\
   \bar g_1 &= b_v \bar f_v,
    \quad
    \delta g_1  = b_v
    \\
   \bar g_2 &= b_v \bar f_v + \bar k_{4F} \Theta,
    \quad
    (\delta g_{2_F} , \delta g_{2_T}) = (b_v,  \lr{ p_{4F}  \bar k_{4F}  \Theta })
    \\
    \bar g_3 &= \bar k_{4R} + \bar k_3,
    \quad
    \delta g_3 = \lr{ p_{4R} \bar k_{4R} + p_3 \bar k_3}
    \\
    \bar g_{23} &= \bar k_{4R} b_v,
    \quad
    \delta g_{23}  = \lr{ p_{4R} \bar k_{4R} b_v }
    \\
    \bar g_{32} &= \bar k_{4F} V \Theta,
    \quad
    \delta g_{32}  = \lr{ p_{4F} \bar k_{4F} V \Theta }
    \\
    \bar b_{11} &= b_v \bar f_v,
    \quad
    \delta b_{11}  = b_v
    \\
    \bar b_{42} &= \frac{\omega_u b_u}{\bar f_v},
    \quad
    \delta b_{42}  = -\lr{\frac{\omega_u b_u}{\bar f_v^2}}
\end{align*}
\end{minipage}

\end{itemize}
